proofs/fstar/extraction/Libcrux.Kem.Kyber.Hash_functions.fsti
@@ -14,25 +14,24 @@ val v_PRF (v_LEN: usize) (input: t_Slice u8)
 
 let v_THREE_BLOCKS: usize = v_BLOCK_SIZE *! sz 3
 
-type t_Shake128State (v_K: usize) = {
-  f_state:t_Array Libcrux.Hacl.Sha3.Incremental.t_Shake128State v_K
-}
+val free (xof_state: Libcrux.Hacl.Sha3.Incremental_x4.t_Shake128StateX4)
+    : Prims.Pure Prims.unit Prims.l_True (fun _ -> Prims.l_True)
 
-val impl__new: v_K: usize -> Prims.unit
-  -> Prims.Pure (t_Shake128State v_K) Prims.l_True (fun _ -> Prims.l_True)
-
-val absorb (v_K: usize) (input: t_Array (t_Array u8 (sz 34)) v_K)
-    : Prims.Pure (t_Shake128State v_K) Prims.l_True (fun _ -> Prims.l_True)
-
-val free (v_K: usize) (xof_state: t_Shake128State v_K)
-    : Prims.Pure (t_Shake128State v_K) Prims.l_True (fun _ -> Prims.l_True)
-
-val squeeze_block (v_K: usize) (xof_state: t_Shake128State v_K)
-    : Prims.Pure (t_Shake128State v_K & t_Array (t_Array u8 (sz 168)) v_K)
+val squeeze_block (v_K: usize) (xof_state: Libcrux.Hacl.Sha3.Incremental_x4.t_Shake128StateX4)
+    : Prims.Pure
+      (Libcrux.Hacl.Sha3.Incremental_x4.t_Shake128StateX4 & t_Array (t_Array u8 (sz 168)) v_K)
       Prims.l_True
       (fun _ -> Prims.l_True)
 
-val squeeze_three_blocks (v_K: usize) (xof_state: t_Shake128State v_K)
-    : Prims.Pure (t_Shake128State v_K & t_Array (t_Array u8 (sz 504)) v_K)
+val squeeze_three_blocks
+      (v_K: usize)
+      (xof_state: Libcrux.Hacl.Sha3.Incremental_x4.t_Shake128StateX4)
+    : Prims.Pure
+      (Libcrux.Hacl.Sha3.Incremental_x4.t_Shake128StateX4 & t_Array (t_Array u8 (sz 504)) v_K)
+      Prims.l_True
+      (fun _ -> Prims.l_True)
+
+val absorb (v_K: usize) (input: t_Array (t_Array u8 (sz 34)) v_K)
+    : Prims.Pure Libcrux.Hacl.Sha3.Incremental_x4.t_Shake128StateX4
       Prims.l_True
       (fun _ -> Prims.l_True)
